txn-data-consistency/CCv_Eiger_Port_plus.thy
@@ -150,6 +150,11 @@ definition get_ctx :: "'v state \<Rightarrow> (key \<rightharpoonup> ('v \<times
     \<exists>cts v rs. wtxn_state (svrs s k) t = Commit cts v rs deps \<and>
     kvt_map k = Some (v, t)}"
 
+definition get_ctx' :: "'v state \<Rightarrow> cl_id \<Rightarrow> ctx_kt" where
+  "get_ctx' s cl \<equiv> \<Union>{insert (k, t) deps | k t deps.
+    \<exists>cts v rs. wtxn_state (svrs s k) t = Commit cts v rs deps \<and>
+     t = read_at (wtxn_state (svrs s k)) (gst (cls s cl)) cl}"
+
 definition view_of :: "(key \<Rightarrow> txid list) \<Rightarrow> ctx_kt \<Rightarrow> view" where
   "view_of corder u \<equiv> (\<lambda>k. {THE i. i < length (corder k) \<and> corder k ! i = t
     | t. (k, t) \<in> u \<and> t \<in> set (corder k)})"
